Make VLSM a record, combine non-VLSMType fields into VLSMMachine (#14)
This changes the definition of VLSM from a nested sigT into
a record, and collapses the two records VLSMSign and VLSMClass
into a single VLSMMachine record because that division was never
useful.
(Separating VLSMType from the rest lets us write definitions like
VLSM_incl that can only be applied to two VLSMs with the same
VLSMType, and it was never helpful to talk about two VLSMs with
the same initial messages and states but different transitions.
The other possible use would be if definitions like
pre_loaded_with_all_messages_vlsm could reuse some of the records,
but VLSMClass dependend on VLSMSign and we never wanted to
change just the transition or valid functions while leaving the
initial states or messages alone).

Unfortunately this somehow changed things so that the extremely
limited form of unification used in the `apply` tactic can no longer
directly apply some lemmas to some goals. For example, lemmas with
conclusions about composite_transition no longer work with the
plain `apply` if the goal was (vtransition (free_composite_vlsm IM)),
even though that expression can reduce to composite_transition.

This can usually be fixed by using `rapply`, which is like
`apply` but based on `refine` and uses a less limited unification
algorithm. I now export it from our Preamble (it's from
Coq.Program.Tactics).
If that fails you can also explicitly supply more arguments.

There is not an `rapply lem in H` form, but the special case of
`apply lem in H;assumption.` can become `revert H;rapply lem`.

theories/VLSM/Core/Composition.v
@@ -150,12 +150,12 @@ The next few results describe several properties of the [state_update] operation
     Qed.
   End composite_type.
 
-  Section composite_sig.
-(** ** The signature of a composite VLSM
+  Section sec_composite_vlsm.
+(** ** Constrained VLSM composition
 
 Assume an non-empty <<index>> type and let <<IT>> be
-an <<index>>ed family of [VLSMType]s, and for each index <<i>>, let <<IS i>> be
-a [VLSMSign]ature of type <<IT i>>.
+an <<index>>ed family of [VLSMType]s, and for each index <<i>>, let <<IM i>> be
+a [VLSMMachine] of type <<IT i>>.
 *)
 
 (**
@@ -181,8 +181,8 @@ states have the [initial_state_prop]erty in the corresponding component signatur
       {| inhabitant := composite_s0 |}.
 
 (**
-A message has the [initial_message_prop]erty in the [composite_sig]nature
-iff it has the [initial_message_prop]erty in any of the component signatures.
+A message has the [initial_message_prop]erty in the composite
+iff it has the [initial_message_prop]erty in any of the components.
 *)
     Definition composite_initial_message_prop (m : message) : Prop
       :=
@@ -190,13 +190,6 @@ iff it has the [initial_message_prop]erty in any of the component signatures.
 
     Definition option_composite_initial_message_prop : option message -> Prop
       := from_option composite_initial_message_prop True.
-
-    Definition composite_sig
-      : VLSMSign composite_type
-      :=
-        {|   initial_state_prop := composite_initial_state_prop
-           ; initial_message_prop := composite_initial_message_prop
-        |}.
 
 (**
 We can always "lift" state <<sj>> from component <<j>> to a composite state by
@@ -267,20 +260,10 @@ updating an initial composite state, say [s0], to <<sj>> on component <<j>>.
       - exact input_a.
     Defined.
 
-  End composite_sig.
-
-  Section sec_composite_vlsm.
-(** ** Constrained VLSM composition
-
-Assume an non-empty <<index>> type, let
-<<IT>> be an <<index>>ed family of [VLSMType]s, and for each index <<i>>, let
-<<IS i>> be a [VLSMSign]ature of type <<IT i>> and <<IM i>> be a VLSM of
-signature <<IS i>>.
-*)
-
 (**
-The [transition] function for the [composite_vlsm] is defined as follows
-takes a transition in the VLSM corresponding to the given [composite_label]
+The [transition] function for the [composite_vlsm] takes a transition in
+the component selected by the index in the given [composite_label]
+with the contained label,
 and returnes the produced message together with the state updated on that
 component:
 *)
@@ -326,9 +309,11 @@ the [composite_valid]ity.
 
     Definition composite_vlsm_machine
       (constraint : composite_label -> composite_state * option message -> Prop)
-      : VLSMClass composite_sig
+      : VLSMMachine composite_type
       :=
-      {|  transition := composite_transition
+      {|  initial_state_prop := composite_initial_state_prop
+       ;  initial_message_prop := composite_initial_message_prop
+       ;  transition := composite_transition
        ;  valid := constrained_composite_valid constraint
       |}.
 
@@ -879,7 +864,7 @@ Proof.
       apply valid_state_project_preloaded_to_preloaded.
     + apply any_message_is_valid_in_preloaded.
     + destruct l. apply Hcvalid.
-  - apply composite_transition_project_active in Htrans;assumption.
+  - revert Htrans; rapply composite_transition_project_active.
 Qed.
 
 Lemma input_valid_transition_project_active
@@ -1015,12 +1000,13 @@ Context
   {index : Type}
   {IndEqDec : EqDecision index}
   (IM : index -> VLSM message)
+  (constraint : composite_label IM -> composite_state IM * option message -> Prop)
   {index_listing : list index}
   (finite_index : Listing index_listing).
 
 Lemma composite_decidable_initial_message
   (Hdec_init : forall i, vdecidable_initial_messages_prop (IM i))
-  : decidable_initial_messages_prop (composite_sig IM).
+  : decidable_initial_messages_prop (composite_vlsm_machine IM constraint).
 Proof.
   intro m. simpl. unfold composite_initial_message_prop.
   apply
