theories/VLSM/Lib/Preamble.v
@@ -1,3 +1,5 @@
+From Coq Require Export Program.Tactics.
+Obligation Tactic := idtac.
 From stdpp Require Import prelude.
 From Coq Require Import Eqdep_dec.
 
